WIP

Kinding.v
@@ -154,14 +154,8 @@ Lemma valid_kind_weakening : forall E F G K,
 Proof.
   introv Hv He.
   apply regular_valid_kind in Hv.
-  remember (E & G) as EG.
-  generalize dependent G.
-  generalize dependent F.
-  generalize dependent E.
-  generalize dependent K.
-  generalize dependent EG.
   pose combined_kinding_weakening.
-  intuition assumption.
+  intuition eauto.
 Qed.
 
 Lemma valid_kind_weakening_l : forall E F K,
@@ -181,15 +175,8 @@ Lemma kinding_weakening : forall E F G T K,
 Proof.
   introv Hk He.
   apply regular_kinding in Hk.
-  remember (E & G) as EG.
-  generalize dependent G.
-  generalize dependent F.
-  generalize dependent E.
-  generalize dependent K.
-  generalize dependent T.
-  generalize dependent EG.
   pose combined_kinding_weakening.
-  intuition assumption.
+  intuition eauto.
 Qed.
 
 Lemma kinding_weakening_l : forall E F T K,
@@ -210,18 +197,8 @@ Lemma valid_scheme_vars_weakening : forall E F G M Xs,
 Proof.
   introv Hf Hs He.
   apply regular_valid_scheme_vars in Hs.
-  remember (E & G) as EG.
-  generalize dependent He.
-  generalize dependent HeqEG.
-  generalize dependent Hf.
-  generalize dependent G.
-  generalize dependent F.
-  generalize dependent E.
-  generalize dependent Xs.
-  generalize dependent M.
-  generalize dependent EG.
   pose combined_kinding_weakening.
-  intuition assumption.
+  intuition eauto.
 Qed.
 
 Lemma valid_scheme_vars_weakening_l : forall E F M Xs,
@@ -243,15 +220,9 @@ Lemma valid_scheme_weakening : forall E F G M,
 Proof.
   introv Hs He.
   apply regular_valid_scheme in Hs.
-  remember (E & G) as EG.
-  generalize dependent G.
-  generalize dependent F.
-  generalize dependent E.
-  generalize dependent M.
-  generalize dependent EG.
   pose combined_kinding_weakening.
-  intuition assumption.
-Qed.  
+  intuition eauto.
+Qed.
 
 Lemma valid_scheme_weakening_l : forall E F M,
     valid_scheme E M ->
@@ -270,16 +241,8 @@ Lemma type_equal_core_weakening : forall E F G T1 T2 K,
 Proof.
   introv Hte He.
   apply regular_type_equal_core in Hte.
-  remember (E & G) as EG.
-  generalize dependent G.
-  generalize dependent F.
-  generalize dependent E.
-  generalize dependent K.
-  generalize dependent T2.
-  generalize dependent T1.
-  generalize dependent EG.
   pose combined_kinding_weakening.
-  intuition assumption.
+  intuition eauto.
 Qed.
 
 Lemma type_equal_core_weakening_l : forall E F T1 T2 K,
@@ -299,16 +262,8 @@ Lemma type_equal_cong_weakening : forall E F G T1 T2 K,
 Proof.
   introv Hte He.
   apply regular_type_equal_cong in Hte.
-  remember (E & G) as EG.
-  generalize dependent G.
-  generalize dependent F.
-  generalize dependent E.
-  generalize dependent K.
-  generalize dependent T2.
-  generalize dependent T1.
-  generalize dependent EG.
   pose combined_kinding_weakening.
-  intuition assumption.
+  intuition eauto.
 Qed.
 
 Lemma type_equal_cong_weakening_l : forall E F T1 T2 K,
@@ -328,16 +283,8 @@ Lemma type_equal_symm_weakening : forall E F G T1 T2 K,
 Proof.
   introv Hte He.
   apply regular_type_equal_symm in Hte.
-  remember (E & G) as EG.
-  generalize dependent G.
-  generalize dependent F.
-  generalize dependent E.
-  generalize dependent K.
-  generalize dependent T2.
-  generalize dependent T1.
-  generalize dependent EG.
   pose combined_kinding_weakening.
-  intuition assumption.
+  intuition eauto.
 Qed.
 
 Lemma type_equal_symm_weakening_l : forall E F T1 T2 K,
@@ -357,16 +304,8 @@ Lemma type_equal_weakening : forall E F G T1 T2 K,
 Proof.
   introv Hte He.
   apply regular_type_equal in Hte.
-  remember (E & G) as EG.
-  generalize dependent G.
-  generalize dependent F.
-  generalize dependent E.
-  generalize dependent K.
-  generalize dependent T2.
-  generalize dependent T1.
-  generalize dependent EG.
   pose combined_kinding_weakening.
-  intuition assumption.
+  intuition eauto.
 Qed.
 
 Lemma type_equal_weakening_l : forall E F T1 T2 K,
@@ -386,16 +325,8 @@ Lemma subtype_weakening : forall E F G T1 T2 cs,
 Proof.
   introv Hs He.
   apply regular_subtype in Hs.
-  remember (E & G) as EG.
-  generalize dependent G.
-  generalize dependent F.
-  generalize dependent E.
-  generalize dependent cs.
-  generalize dependent T2.
-  generalize dependent T1.
-  generalize dependent EG.
   pose combined_kinding_weakening.
-  intuition assumption.
+  intuition eauto.
 Qed.
 
 Lemma subtype_weakening_l : forall E F T1 T2 cs,
@@ -1655,9 +1586,9 @@ Inductive valid_kind_validated : env -> knd -> Prop :=
       environment E ->
       type T1 ->
       type T2 ->
-      valid_env E ->
-      kinding E T1 (knd_row CSet.universe) ->
-      kinding E T2 (knd_row CSet.universe) ->
+      valid_env_validated E ->
+      kinding_validated E T1 (knd_row CSet.universe) ->
+      kinding_validated E T2 (knd_row CSet.universe) ->
       valid_kind_validated E (knd_range T1 T2)
 
 with kinding_validated : env -> typ -> knd -> Prop :=
@@ -1666,14 +1597,14 @@ with kinding_validated : env -> typ -> knd -> Prop :=
       binds X (bind_knd K) E ->
       environment E ->
       kind K ->
-      valid_kind E K ->
+      valid_kind_validated E K ->
       kinding_validated E (typ_fvar X) K
   | kinding_validated_constructor : forall E c T cs,
       kinding_validated E T knd_type ->
       cs = CSet.singleton c ->
       environment E ->
       type T ->
-      valid_env E ->
+      valid_env_validated E ->
       kinding_validated E (typ_constructor c T) (knd_row cs)
   | kinding_validated_or : forall E T1 T2 cs1 cs2 cs12,
       kinding_validated E T1 (knd_row cs1) ->
@@ -1685,7 +1616,7 @@ with kinding_validated : env -> typ -> knd -> Prop :=
       type T2 ->
       CSet.Nonempty cs1 ->
       CSet.Nonempty cs2 ->
-      valid_env E ->
+      valid_env_validated E ->
       kinding_validated E (typ_or T1 T2) (knd_row cs12)
   | kinding_validated_proj : forall E T cs cs',
       kinding_validated E T (knd_row cs) ->
@@ -1694,13 +1625,14 @@ with kinding_validated : env -> typ -> knd -> Prop :=
       environment E ->
       type T ->
       CSet.Nonempty cs ->
-      valid_env E ->
+      valid_env_validated E ->
       kinding_validated E (typ_proj T cs') (knd_row cs')
   | kinding_validated_row : forall E T,
       kinding_validated E T (knd_row CSet.universe) ->
       environment E ->
       type T ->
-      valid_env E ->
+      valid_env_validated E ->
+      valid_kind_validated E (knd_range T T) ->
       kinding_validated E (typ_row T) (knd_range T T)
   | kinding_validated_variant : forall E T T1 T2,
       kinding_validated E T (knd_range T1 T2) ->
@@ -1708,10 +1640,10 @@ with kinding_validated : env -> typ -> knd -> Prop :=
       type T ->
       type T1 ->
       type T2 ->
-      valid_env E ->
-      kinding E T1 (knd_row CSet.universe) ->
-      kinding E T2 (knd_row CSet.universe) ->
-      subtype E T2 T1 CSet.universe ->
+      valid_env_validated E ->
+      kinding_validated E T1 (knd_row CSet.universe) ->
+      kinding_validated E T2 (knd_row CSet.universe) ->
+      subtype_validated E T2 T1 CSet.universe ->
       kinding_validated E (typ_variant T) knd_type
   | kinding_validated_arrow : forall E T1 T2,
       kinding_validated E T1 knd_type -> 
@@ -1719,19 +1651,19 @@ with kinding_validated : env -> typ -> knd -> Prop :=
       environment E ->
       type T1 ->
       type T2 ->
-      valid_env E ->
+      valid_env_validated E ->
       kinding_validated E (typ_arrow T1 T2) knd_type
   | kinding_validated_top : forall E cs,
       valid_env_validated E ->
       CSet.Nonempty cs ->
       environment E ->
-      valid_env E ->
+      valid_env_validated E ->
       kinding_validated E (typ_top cs) (knd_row cs)
   | kinding_validated_bot : forall E cs,
       valid_env_validated E ->
       CSet.Nonempty cs ->
       environment E ->
-      valid_env E ->
+      valid_env_validated E ->
       kinding_validated E (typ_bot cs) (knd_row cs)
   | kinding_validated_meet : forall E T1 T2 cs,
       kinding_validated E T1 (knd_row cs) ->
@@ -1740,7 +1672,7 @@ with kinding_validated : env -> typ -> knd -> Prop :=
       type T1 ->
       type T2 ->
       CSet.Nonempty cs ->
-      valid_env E ->
+      valid_env_validated E ->
       kinding_validated E (typ_meet T1 T2) (knd_row cs)
   | kinding_validated_join : forall E T1 T2 cs,
       kinding_validated E T1 (knd_row cs) ->
@@ -1749,7 +1681,7 @@ with kinding_validated : env -> typ -> knd -> Prop :=
       type T1 ->
       type T2 ->
       CSet.Nonempty cs ->
-      valid_env E ->
+      valid_env_validated E ->
       kinding_validated E (typ_join T1 T2) (knd_row cs)
   | kinding_validated_range_subsumption : forall E T T1 T2 T1' T2',
       kinding_validated E T (knd_range T1 T2) ->
@@ -1761,13 +1693,15 @@ with kinding_validated : env -> typ -> knd -> Prop :=
       type T2 ->
       type T1' ->
       type T2' ->
-      valid_env E ->
-      kinding E T1 (knd_row CSet.universe) ->
-      kinding E T1' (knd_row CSet.universe) ->
-      kinding E T2 (knd_row CSet.universe) ->
-      kinding E T2' (knd_row CSet.universe) ->
-      subtype E T2 T1 CSet.universe ->
-      subtype E T2' T1' CSet.universe ->
+      valid_env_validated E ->
+      kinding_validated E T1 (knd_row CSet.universe) ->
+      kinding_validated E T1' (knd_row CSet.universe) ->
+      kinding_validated E T2 (knd_row CSet.universe) ->
+      kinding_validated E T2' (knd_row CSet.universe) ->
+      subtype_validated E T2 T1 CSet.universe ->
+      subtype_validated E T2' T1' CSet.universe ->
+      valid_kind_validated E (knd_range T1 T2) ->
+      valid_kind_validated E (knd_range T1' T2') ->
       kinding_validated E T (knd_range T1' T2')
 
 with valid_scheme_vars_validated : env -> sch -> list var -> Prop :=
@@ -1775,7 +1709,7 @@ with valid_scheme_vars_validated : env -> sch -> list var -> Prop :=
       kinding_validated E T knd_type ->
       environment E ->
       type T ->
-      valid_env E ->
+      valid_env_validated E ->
       valid_scheme_vars_validated E (sch_empty T) nil
   | valid_scheme_vars_validated_bind : forall X Xs E K M,
       valid_kind_validated E K ->
@@ -1785,8 +1719,8 @@ with valid_scheme_vars_validated : env -> sch -> list var -> Prop :=
       kind K ->
       scheme_vars (M ^ X) Xs ->
       scheme_vars (sch_bind K M) (X :: Xs) ->
-      valid_env E ->
-      valid_env (E & X ~:: K) ->
+      valid_env_validated E ->
+      valid_env_validated (E & X ~:: K) ->
       valid_scheme_vars_validated E (sch_bind K M) (X :: Xs)
 
 with valid_scheme_validated : env -> sch -> Prop :=
@@ -1796,7 +1730,7 @@ with valid_scheme_validated : env -> sch -> Prop :=
           valid_scheme_vars_validated E M Xs) ->
       environment E ->
       scheme M ->
-      valid_env E ->
+      valid_env_validated E ->
       valid_scheme_validated E M
 
 with valid_env_validated : env -> Prop :=
@@ -1831,7 +1765,7 @@ with type_equal_core_validated : env -> typ -> typ -> knd -> Prop :=
       type T2 ->
       CSet.Nonempty cs1 ->
       CSet.Nonempty cs2 ->
-      valid_env E ->
+      valid_env_validated E ->
       type_equal_core_validated E
         (typ_or T1 T2) (typ_or T2 T1) (knd_row cs12)
   | type_equal_core_validated_or_associative :
@@ -1850,7 +1784,7 @@ with type_equal_core_validated : env -> typ -> typ -> knd -> Prop :=
       CSet.Nonempty cs1 ->
       CSet.Nonempty cs2 ->
       CSet.Nonempty cs3 ->
-      valid_env E ->
+      valid_env_validated E ->
       type_equal_core_validated E
         (typ_or T1 (typ_or T2 T3)) (typ_or (typ_or T1 T2) T3)
         (knd_row cs123)
@@ -1889,7 +1823,7 @@ with type_equal_core_validated : env -> typ -> typ -> knd -> Prop :=
       type T4 ->
       CSet.Nonempty cs1 ->
       CSet.Nonempty cs2 ->
-      valid_env E ->
+      valid_env_validated E ->
       type_equal_core_validated E
         (typ_or (typ_meet T1 T3) (typ_meet T2 T4))
         (typ_meet (typ_or T1 T2) (typ_or T3 T4))
@@ -1909,7 +1843,7 @@ with type_equal_core_validated : env -> typ -> typ -> knd -> Prop :=
       type T4 ->
       CSet.Nonempty cs1 ->
       CSet.Nonempty cs2 ->
-      valid_env E ->
+      valid_env_validated E ->
       type_equal_core_validated E
         (typ_or (typ_join T1 T3) (typ_join T2 T4))
         (typ_join (typ_or T1 T2) (typ_or T3 T4))
@@ -1925,7 +1859,7 @@ with type_equal_core_validated : env -> typ -> typ -> knd -> Prop :=
       environment E ->
       type T ->
       CSet.Nonempty cs1 ->
-      valid_env E ->
+      valid_env_validated E ->
       type_equal_core_validated E
         (typ_or (typ_proj T cs2) (typ_proj T cs3))
         (typ_proj T cs23)
@@ -1935,7 +1869,7 @@ with type_equal_core_validated : env -> typ -> typ -> knd -> Prop :=
       environment E ->
       type T ->
       CSet.Nonempty cs ->
-      valid_env E ->
+      valid_env_validated E ->
       type_equal_core_validated E (typ_proj T cs) T (knd_row cs)
   | type_equal_core_validated_proj_or_l : forall E T1 T2 cs1 cs1' cs2,
       kinding_validated E T1 (knd_row cs1) ->
@@ -1948,7 +1882,7 @@ with type_equal_core_validated : env -> typ -> typ -> knd -> Prop :=
       type T2 ->
       CSet.Nonempty cs1 ->
       CSet.Nonempty cs2 ->
-      valid_env E ->
+      valid_env_validated E ->
       type_equal_core_validated E
         (typ_proj (typ_or T1 T2) cs1') (typ_proj T1 cs1')
         (knd_row cs1')
@@ -1963,7 +1897,7 @@ with type_equal_core_validated : env -> typ -> typ -> knd -> Prop :=
       type T2 ->
       CSet.Nonempty cs1 ->
       CSet.Nonempty cs2 ->
-      valid_env E ->
+      valid_env_validated E ->
       type_equal_core_validated E
         (typ_proj (typ_or T1 T2) cs2') (typ_proj T2 cs2')
         (knd_row cs2')
@@ -1982,7 +1916,7 @@ with type_equal_core_validated : env -> typ -> typ -> knd -> Prop :=
       type T2 ->
       CSet.Nonempty cs1 ->
       CSet.Nonempty cs2 ->
-      valid_env E ->
+      valid_env_validated E ->
       type_equal_core_validated E
         (typ_proj (typ_or T1 T2) cs12')
         (typ_or (typ_proj T1 cs1') (typ_proj T2 cs2'))
@@ -1996,7 +1930,7 @@ with type_equal_core_validated : env -> typ -> typ -> knd -> Prop :=
       type T1 ->
       type T2 ->
       CSet.Nonempty cs ->
-      valid_env E ->
+      valid_env_validated E ->
       type_equal_core_validated E
         (typ_proj (typ_meet T1 T2) cs')
         (typ_meet (typ_proj T1 cs') (typ_proj T2 cs'))
@@ -2010,7 +1944,7 @@ with type_equal_core_validated : env -> typ -> typ -> knd -> Prop :=
       type T1 ->
       type T2 ->
       CSet.Nonempty cs ->
-      valid_env E ->
+      valid_env_validated E ->
       type_equal_core_validated E
         (typ_proj (typ_join T1 T2) cs')
         (typ_join (typ_proj T1 cs') (typ_proj T2 cs'))
@@ -2022,7 +1956,7 @@ with type_equal_core_validated : env -> typ -> typ -> knd -> Prop :=
       type T1 ->
       type T2 ->
       CSet.Nonempty cs ->
-      valid_env E ->
+      valid_env_validated E ->
       type_equal_core_validated E
         (typ_meet T1 T2) (typ_meet T2 T1) (knd_row cs)
   | type_equal_core_validated_meet_associative : forall E T1 T2 T3 cs,
@@ -2034,7 +1968,7 @@ with type_equal_core_validated : env -> typ -> typ -> knd -> Prop :=
       type T2 ->
       type T3 ->
       CSet.Nonempty cs ->
-      valid_env E ->
+      valid_env_validated E ->
       type_equal_core_validated E
         (typ_meet T1 (typ_meet T2 T3))
         (typ_meet (typ_meet T1 T2) T3)
@@ -2044,7 +1978,7 @@ with type_equal_core_validated : env -> typ -> typ -> knd -> Prop :=
       environment E ->
       type T1 ->
       CSet.Nonempty cs ->
-      valid_env E ->
+      valid_env_validated E ->
       type_equal_core_validated E
         (typ_meet T1 (typ_top cs)) T1 (knd_row cs)
   | type_equal_core_validated_meet_absorption : forall E T1 T2 cs,
@@ -2054,7 +1988,7 @@ with type_equal_core_validated : env -> typ -> typ -> knd -> Prop :=
       type T1 ->
       type T2 ->
       CSet.Nonempty cs ->
-      valid_env E ->
+      valid_env_validated E ->
       type_equal_core_validated E
         (typ_meet T1 (typ_join T1 T2)) T1 (knd_row cs)
   | type_equal_core_validated_meet_distribution :
@@ -2067,7 +2001,7 @@ with type_equal_core_validated : env -> typ -> typ -> knd -> Prop :=
       type T2 ->
       type T3 ->
       CSet.Nonempty cs ->
-      valid_env E ->
+      valid_env_validated E ->
       type_equal_core_validated E
         (typ_meet T1 (typ_join T2 T3))
         (typ_join (typ_meet T1 T2) (typ_meet T1 T3))
@@ -2079,7 +2013,7 @@ with type_equal_core_validated : env -> typ -> typ -> knd -> Prop :=
       type T1 ->
       type T2 ->
       CSet.Nonempty cs ->
-      valid_env E ->
+      valid_env_validated E ->
       type_equal_core_validated E
         (typ_join T1 T2) (typ_join T2 T1) (knd_row cs)
   | type_equal_core_validated_join_associative : forall E T1 T2 T3 cs,
@@ -2091,7 +2025,7 @@ with type_equal_core_validated : env -> typ -> typ -> knd -> Prop :=
       type T2 ->
       type T3 ->
       CSet.Nonempty cs ->
-      valid_env E ->
+      valid_env_validated E ->
       type_equal_core_validated E
         (typ_join T1 (typ_join T2 T3))
         (typ_join (typ_join T1 T2) T3)
@@ -2101,7 +2035,7 @@ with type_equal_core_validated : env -> typ -> typ -> knd -> Prop :=
       environment E ->
       type T1 ->
       CSet.Nonempty cs ->
-      valid_env E ->
+      valid_env_validated E ->
       type_equal_core_validated E
         (typ_join T1 (typ_bot cs)) T1 (knd_row cs)
   | type_equal_core_validated_join_absorption : forall E T1 T2 cs,
@@ -2111,7 +2045,7 @@ with type_equal_core_validated : env -> typ -> typ -> knd -> Prop :=
       type T1 ->
       type T2 ->
       CSet.Nonempty cs ->
-      valid_env E ->
+      valid_env_validated E ->
       type_equal_core_validated E
         (typ_join T1 (typ_meet T1 T2)) T1 (knd_row cs)
   | type_equal_core_validated_join_distribution :
@@ -2124,7 +2058,7 @@ with type_equal_core_validated : env -> typ -> typ -> knd -> Prop :=
       type T2 ->
       type T3 ->
       CSet.Nonempty cs ->
-      valid_env E ->
+      valid_env_validated E ->
       type_equal_core_validated E
         (typ_join T1 (typ_meet T2 T3))
         (typ_meet (typ_join T1 T2) (typ_join T1 T3))
@@ -2137,9 +2071,9 @@ with type_equal_cong_validated : env -> typ -> typ -> knd -> Prop :=
       environment E ->
       type T1 ->
       type T1' ->
-      valid_env E ->
-      kinding E T1 knd_type ->
-      kinding E T1' knd_type ->
+      valid_env_validated E ->
+      kinding_validated E T1 knd_type ->
+      kinding_validated E T1' knd_type ->
       type_equal_cong_validated E
         (typ_constructor c T1) (typ_constructor c T1')
         (knd_row cs)
@@ -2154,9 +2088,9 @@ with type_equal_cong_validated : env -> typ -> typ -> knd -> Prop :=
       type T2 ->
       CSet.Nonempty cs1 ->
       CSet.Nonempty cs2 ->
-      valid_env E ->
-      kinding E T1 (knd_row cs1) ->
-      kinding E T1' (knd_row cs1) ->
+      valid_env_validated E ->
+      kinding_validated E T1 (knd_row cs1) ->
+      kinding_validated E T1' (knd_row cs1) ->
       type_equal_cong_validated E
         (typ_or T1 T2) (typ_or T1' T2) (knd_row cs12)
   | type_equal_cong_validated_or_r : forall E T1 T2 T2' cs1 cs2 cs12,
@@ -2170,9 +2104,9 @@ with type_equal_cong_validated : env -> typ -> typ -> knd -> Prop :=
       type T2' ->
       CSet.Nonempty cs1 ->
       CSet.Nonempty cs2 ->
-      valid_env E ->
-      kinding E T2 (knd_row cs2) ->
-      kinding E T2' (knd_row cs2) ->
+      valid_env_validated E ->
+      kinding_validated E T2 (knd_row cs2) ->
+      kinding_validated E T2' (knd_row cs2) ->
       type_equal_cong_validated E
         (typ_or T1 T2) (typ_or T1 T2') (knd_row cs12)
   | type_equal_cong_validated_row : forall E T1 T1',
@@ -2180,9 +2114,11 @@ with type_equal_cong_validated : env -> typ -> typ -> knd -> Prop :=
       environment E ->
       type T1 ->
       type T1' ->
-      valid_env E ->
-      kinding E T1 (knd_row CSet.universe) ->
-      kinding E T1' (knd_row CSet.universe) ->
+      valid_env_validated E ->
+      kinding_validated E T1 (knd_row CSet.universe) ->
+      kinding_validated E T1' (knd_row CSet.universe) ->
+      kinding_validated E (typ_row T1') (knd_range T1 T1) ->
+      valid_kind_validated E (knd_range T1 T1) ->
       type_equal_cong_validated E
         (typ_row T1) (typ_row T1') (knd_range T1 T1)
   | type_equal_cong_validated_variant : forall E T1 T1' T2 T3,
@@ -2192,12 +2128,12 @@ with type_equal_cong_validated : env -> typ -> typ -> knd -> Prop :=
       type T1' ->
       type T2 ->
       type T3 ->
-      valid_env E ->
-      kinding E T1 (knd_range T2 T3) ->
-      kinding E T1' (knd_range T2 T3) ->
-      kinding E T2 (knd_row CSet.universe) ->
-      kinding E T3 (knd_row CSet.universe) ->
-      subtype E T3 T2 CSet.universe ->
+      valid_env_validated E ->
+      kinding_validated E T1 (knd_range T2 T3) ->
+      kinding_validated E T1' (knd_range T2 T3) ->
+      kinding_validated E T2 (knd_row CSet.universe) ->
+      kinding_validated E T3 (knd_row CSet.universe) ->
+      subtype_validated E T3 T2 CSet.universe ->
       type_equal_cong_validated E
         (typ_variant T1) (typ_variant T1') knd_type
   | type_equal_cong_validated_arrow_l : forall E T1 T1' T2,
@@ -2207,9 +2143,9 @@ with type_equal_cong_validated : env -> typ -> typ -> knd -> Prop :=
       type T1 ->
       type T1' ->
       type T2 ->
-      valid_env E ->
-      kinding E T1 knd_type ->
-      kinding E T1' knd_type ->
+      valid_env_validated E ->
+      kinding_validated E T1 knd_type ->
+      kinding_validated E T1' knd_type ->
       type_equal_cong_validated E
         (typ_arrow T1 T2) (typ_arrow T1' T2) knd_type
   | type_equal_cong_validated_arrow_r : forall E T1 T2 T2',
@@ -2219,9 +2155,9 @@ with type_equal_cong_validated : env -> typ -> typ -> knd -> Prop :=
       type T1 ->
       type T2 ->
       type T2' ->
-      valid_env E ->
-      kinding E T2 knd_type ->
-      kinding E T2' knd_type ->
+      valid_env_validated E ->
+      kinding_validated E T2 knd_type ->
+      kinding_validated E T2' knd_type ->
       type_equal_cong_validated E
         (typ_arrow T1 T2) (typ_arrow T1 T2') knd_type
   | type_equal_cong_validated_meet_l : forall E T1 T1' T2 cs,
@@ -2232,9 +2168,9 @@ with type_equal_cong_validated : env -> typ -> typ -> knd -> Prop :=
       type T1' ->
       type T2 ->
       CSet.Nonempty cs ->
-      valid_env E ->
-      kinding E T1 (knd_row cs) ->
-      kinding E T1' (knd_row cs) ->
+      valid_env_validated E ->
+      kinding_validated E T1 (knd_row cs) ->
+      kinding_validated E T1' (knd_row cs) ->
       type_equal_cong_validated E
         (typ_meet T1 T2) (typ_meet T1' T2) (knd_row cs)
   | type_equal_cong_validated_meet_r : forall E T1 T2 T2' cs,
@@ -2245,9 +2181,9 @@ with type_equal_cong_validated : env -> typ -> typ -> knd -> Prop :=
       type T2 ->
       type T2' ->
       CSet.Nonempty cs ->
-      valid_env E ->
-      kinding E T2 (knd_row cs) ->
-      kinding E T2' (knd_row cs) ->
+      valid_env_validated E ->
+      kinding_validated E T2 (knd_row cs) ->
+      kinding_validated E T2' (knd_row cs) ->
       type_equal_cong_validated E
         (typ_meet T1 T2) (typ_meet T1 T2') (knd_row cs)
   | type_equal_cong_validated_join_l : forall E T1 T1' T2 cs,
@@ -2258,9 +2194,9 @@ with type_equal_cong_validated : env -> typ -> typ -> knd -> Prop :=
       type T1' ->
       type T2 ->
       CSet.Nonempty cs ->
-      valid_env E ->
-      kinding E T1 (knd_row cs) ->
-      kinding E T1' (knd_row cs) ->
+      valid_env_validated E ->
+      kinding_validated E T1 (knd_row cs) ->
+      kinding_validated E T1' (knd_row cs) ->
       type_equal_cong_validated E
         (typ_join T1 T2) (typ_join T1' T2) (knd_row cs)
   | type_equal_cong_validated_join_r : forall E T1 T2 T2' cs,
@@ -2271,9 +2207,9 @@ with type_equal_cong_validated : env -> typ -> typ -> knd -> Prop :=
       type T2 ->
       type T2' ->
       CSet.Nonempty cs ->
-      valid_env E ->
-      kinding E T2 (knd_row cs) ->
-      kinding E T2' (knd_row cs) ->
+      valid_env_validated E ->
+      kinding_validated E T2 (knd_row cs) ->
+      kinding_validated E T2' (knd_row cs) ->
       type_equal_cong_validated E
         (typ_join T1 T2) (typ_join T1 T2') (knd_row cs)
   | type_equal_cong_validated_range_subsumption :
@@ -2288,15 +2224,17 @@ with type_equal_cong_validated : env -> typ -> typ -> knd -> Prop :=
       type T3' ->
       type T4 ->
       type T4' ->
-      valid_env E ->
-      kinding E T1 (knd_range T3 T4) ->
-      kinding E T2 (knd_range T3 T4) ->
-      kinding E T3 (knd_row CSet.universe) ->
-      kinding E T3' (knd_row CSet.universe) ->
-      kinding E T4 (knd_row CSet.universe) ->
-      kinding E T4' (knd_row CSet.universe) ->
-      subtype E T4 T3 CSet.universe ->
-      subtype E T4' T3' CSet.universe ->
+      valid_env_validated E ->
+      kinding_validated E T1 (knd_range T3 T4) ->
+      kinding_validated E T2 (knd_range T3 T4) ->
+      kinding_validated E T3 (knd_row CSet.universe) ->
+      kinding_validated E T3' (knd_row CSet.universe) ->
+      kinding_validated E T4 (knd_row CSet.universe) ->
+      kinding_validated E T4' (knd_row CSet.universe) ->
+      subtype_validated E T4 T3 CSet.universe ->
+      subtype_validated E T4' T3' CSet.universe ->
+      valid_kind_validated E (knd_range T3 T4) ->
+      valid_kind_validated E (knd_range T3' T4') ->
       type_equal_cong_validated E T1 T2 (knd_range T3' T4')
   | type_equal_cong_validated_core : forall E T1 T1' K,
       type_equal_core_validated E T1 T1' K ->
@@ -2304,10 +2242,10 @@ with type_equal_cong_validated : env -> typ -> typ -> knd -> Prop :=
       type T1 ->
       type T1' ->
       kind K ->
-      valid_env E ->
-      kinding E T1 K ->
-      kinding E T1' K ->
-      valid_kind E K ->
+      valid_env_validated E ->
+      kinding_validated E T1 K ->
+      kinding_validated E T1' K ->
+      valid_kind_validated E K ->
       type_equal_cong_validated E T1 T1' K
 
 with type_equal_symm_validated : env -> typ -> typ -> knd -> Prop :=
@@ -2317,10 +2255,10 @@ with type_equal_symm_validated : env -> typ -> typ -> knd -> Prop :=
       type T1 ->
       type T2 ->
       kind K ->
-      valid_env E ->
-      kinding E T1 K ->
-      kinding E T2 K ->
-      valid_kind E K ->
+      valid_env_validated E ->
+      kinding_validated E T1 K ->
+      kinding_validated E T2 K ->
+      valid_kind_validated E K ->
       type_equal_symm_validated E T1 T2 K
   | type_equal_symm_validated_r : forall E T1 T2 K,
       type_equal_cong_validated E T1 T2 K ->
@@ -2328,10 +2266,10 @@ with type_equal_symm_validated : env -> typ -> typ -> knd -> Prop :=
       type T1 ->
       type T2 ->
       kind K ->
-      valid_env E ->
-      kinding E T1 K ->
-      kinding E T2 K ->
-      valid_kind E K ->
+      valid_env_validated E ->
+      kinding_validated E T1 K ->
+      kinding_validated E T2 K ->
+      valid_kind_validated E K ->
       type_equal_symm_validated E T2 T1 K
 
 with type_equal_validated : env -> typ -> typ -> knd -> Prop :=
@@ -2340,8 +2278,8 @@ with type_equal_validated : env -> typ -> typ -> knd -> Prop :=
       environment E ->
       type T ->
       kind K ->
-      valid_env E ->
-      valid_kind E K ->
+      valid_env_validated E ->
+      valid_kind_validated E K ->
       type_equal_validated E T T K
   | type_equal_validated_step : forall E T1 T2 T3 K,
       type_equal_symm_validated E T1 T2 K ->
@@ -2351,11 +2289,11 @@ with type_equal_validated : env -> typ -> typ -> knd -> Prop :=
       type T2 ->
       type T3 ->
       kind K ->
-      valid_env E ->
-      kinding E T1 K ->
-      kinding E T2 K ->
-      kinding E T3 K ->
-      valid_kind E K ->
+      valid_env_validated E ->
+      kinding_validated E T1 K ->
+      kinding_validated E T2 K ->
+      kinding_validated E T3 K ->
+      valid_kind_validated E K ->
       type_equal_validated E T1 T3 K
 
 with subtype_validated : env -> typ -> typ -> cset -> Prop :=
@@ -2365,9 +2303,9 @@ with subtype_validated : env -> typ -> typ -> cset -> Prop :=
       type T1 ->
       type T2 ->
       CSet.Nonempty cs ->
-      valid_env E ->
-      kinding E T1 (knd_row cs) ->
-      kinding E T2 (knd_row cs) ->
+      valid_env_validated E ->
+      kinding_validated E T1 (knd_row cs) ->
+      kinding_validated E T2 (knd_row cs) ->
       subtype_validated E T1 T2 cs.
 
 Scheme valid_kind_validated_mutind :=
@@ -2513,7 +2451,7 @@ Hint Resolve unvalidated_subtype.
 
 Lemma valid_kind_validated_inv : forall E K,
     valid_kind_validated E K ->
-    valid_env E.
+    valid_env_validated E.
 Proof.
   introv Hv.
   induction Hv; auto.
@@ -2545,18 +2483,25 @@ Hint Extern 1 (CSet.Nonempty ?cs) =>
       inversion Hknd; assumption
   end : valid_kind_regular.
 
-Hint Extern 1 (valid_env ?E) =>
+Hint Extern 1 (valid_env_validated ?E) =>
   match goal with
   | H : valid_kind_validated E _ |- _ =>
       apply (valid_kind_validated_inv H)
   end : valid_kind_validated.
 
+Hint Extern 1 (valid_env ?E) =>
+  match goal with
+  | H : valid_kind_validated E _ |- _ =>
+      apply (unvalidated_valid_env (valid_kind_validated_inv H))
+  end : valid_kind_validated.
+
 Lemma kinding_validated_inv : forall E T K,
     kinding_validated E T K ->
-    valid_env E /\ valid_kind E K.
+    valid_env_validated E /\ valid_kind_validated E K.
 Proof.
   introv Hk.
-  split; destruct Hk; auto using raw_subtype_reflexive with csetdec.
+  split; destruct Hk;
+    auto with valid_kind_validated csetdec.
 Qed.
 
 Hint Constructors kinding_validated : kinding_validated.
@@ -2592,21 +2537,33 @@ Hint Extern 1 (CSet.Nonempty ?cs) =>
       inversion Hknd; assumption
   end : kinding_regular.
 
-Hint Extern 1 (valid_env ?E) =>
+Hint Extern 1 (valid_env_validated ?E) =>
   match goal with
   | H : kinding_validated E _ _ |- _ =>
       apply (proj1 (kinding_validated_inv H))
   end : kinding_validated.
 
-Hint Extern 1 (valid_kind ?E ?K) =>
+Hint Extern 1 (valid_kind_validated ?E ?K) =>
   match goal with
   | H : kinding_validated E _ K |- _ =>
       apply (proj2 (kinding_validated_inv H))
   end : kinding_validated.
 
+Hint Extern 1 (valid_env ?E) =>
+  match goal with
+  | H : kinding_validated E _ _ |- _ =>
+      apply (unvalidated_valid_env (proj1 (kinding_validated_inv H)))
+  end : kinding_validated.
+
+Hint Extern 1 (valid_kind ?E ?K) =>
+  match goal with
+  | H : kinding_validated E _ K |- _ =>
+      apply (unvalidated_valid_kind (proj2 (kinding_validated_inv H)))
+  end : kinding_validated.
+
 Lemma valid_scheme_vars_validated_inv : forall E M Xs,
     valid_scheme_vars_validated E M Xs ->
-    valid_env E.
+    valid_env_validated E.
 Proof.
   introv Hs.
   destruct Hs; auto.
@@ -2631,15 +2588,22 @@ Hint Extern 1 (scheme_vars ?M ?Xs) =>
                   (unvalidated_valid_scheme_vars H))))
   end : valid_scheme_vars_regular.
 
-Hint Extern 1 (valid_env ?E) =>
+Hint Extern 1 (valid_env_validated ?E) =>
   match goal with
   | H : valid_scheme_vars_validated E _ _ |- _ =>
       apply (valid_scheme_vars_validated_inv H)
   end : valid_scheme_vars_validated.
 
+Hint Extern 1 (valid_env ?E) =>
+  match goal with
+  | H : valid_scheme_vars_validated E _ _ |- _ =>
+      apply (unvalidated_valid_env
+               (valid_scheme_vars_validated_inv H))
+  end : valid_scheme_vars_validated.
+
 Lemma valid_scheme_validated_inv : forall E M,
     valid_scheme_validated E M ->
-    valid_env E.
+    valid_env_validated E.
 Proof.
   introv Hs.
   destruct Hs; auto.
@@ -2661,10 +2625,16 @@ Hint Extern 1 (scheme ?M) =>
                (regular_valid_scheme (unvalidated_valid_scheme H))))
   end : valid_scheme_regular.
 
-Hint Extern 1 (valid_env ?E) =>
+Hint Extern 1 (valid_env_validated ?E) =>
   match goal with
   | H : valid_scheme_validated E _ |- _ =>
       apply (valid_scheme_validated_inv H)
+  end : valid_scheme_validated.
+
+Hint Extern 1 (valid_env ?E) =>
+  match goal with
+  | H : valid_scheme_validated E _ |- _ =>
+      apply (unvalidated_valid_env (valid_scheme_validated_inv H))
   end : valid_scheme_validated.
 
 Hint Constructors valid_env_validated : valid_env_validated.
@@ -2678,35 +2648,44 @@ Hint Extern 1 (environment ?E) =>
 
 Lemma type_equal_core_validated_inv : forall E T1 T2 K,
     type_equal_core_validated E T1 T2 K ->
-    valid_env E /\ kinding E T1 K /\ kinding E T2 K /\ valid_kind E K.
+    valid_env_validated E
+    /\ kinding_validated E T1 K
+    /\ kinding_validated E T2 K
+    /\ valid_kind_validated E K.
 Proof.
   introv Hte.
   destruct Hte; subst; splits;
     auto;
-    econstr eapply unvalidated_kinding
-      then solve [eauto|auto with csetdec].
-  - apply kinding_or
+    econstr solve
+     [ auto with kinding_validated
+     | csetdec
+     | eauto with kinding_validated ].
+  - apply kinding_validated_or
       with (cs1 := cs1) (cs2 := CSet.union cs2 cs3);
       auto with csetdec.
-    apply kinding_or
+    apply kinding_validated_or
       with (cs1 := cs2) (cs2 := cs3); auto.
-  - apply kinding_or
+  - apply kinding_validated_or
       with (cs1 := CSet.union cs1 cs2) (cs2 := cs3);
       auto with csetdec.
-    apply kinding_or
+    apply kinding_validated_or
       with (cs1 := cs1) (cs2 := cs2); auto.
-  - apply kinding_proj with (cs := CSet.union cs1 cs2);
+  - apply kinding_validated_proj with (cs := CSet.union cs1 cs2);
       auto with csetdec.
-    apply kinding_or with (cs1 := cs1) (cs2 := cs2);
+    apply kinding_validated_or with (cs1 := cs1) (cs2 := cs2);
       auto.
-  - apply kinding_proj with (cs := CSet.union cs1 cs2);
+  - apply kinding_validated_proj with (cs := CSet.union cs1 cs2);
       auto with csetdec.
-    apply kinding_or with (cs1 := cs1) (cs2 := cs2);
+    apply kinding_validated_or with (cs1 := cs1) (cs2 := cs2);
       auto.
-  - apply kinding_or with (cs1 := cs1') (cs2 := cs2');
+  - apply kinding_validated_proj with (cs := CSet.union cs1 cs2);
       auto with csetdec.
-    + apply kinding_proj with (cs := cs1); auto.
-    + apply kinding_proj with (cs := cs2); auto.
+    apply kinding_validated_or with (cs1 := cs1) (cs2 := cs2);
+      auto.
+  - apply kinding_validated_or with (cs1 := cs1') (cs2 := cs2');
+      auto with csetdec.
+    + apply kinding_validated_proj with (cs := cs1); auto.
+    + apply kinding_validated_proj with (cs := cs2); auto.
 Qed.
 
 Hint Constructors type_equal_core_validated
@@ -2746,13 +2725,13 @@ Hint Extern 1 (CSet.Nonempty ?cs) =>
       inversion Hknd; assumption
   end : type_equal_core_regular.
 
-Hint Extern 1 (valid_env ?E) =>
+Hint Extern 1 (valid_env_validated ?E) =>
   match goal with
   | H : type_equal_core_validated E _ _ _ |- _ =>
       apply (proj41 (type_equal_core_validated_inv H))
-  end : type_equal_core_regular.
+  end : type_equal_core_validated.
 
-Hint Extern 1 (kinding ?E ?T ?K) =>
+Hint Extern 1 (kinding_validated ?E ?T ?K) =>
   match goal with
   | H : type_equal_core_validated E T _ K |- _ =>
       apply (proj42 (type_equal_core_validated_inv H))
@@ -2760,23 +2739,47 @@ Hint Extern 1 (kinding ?E ?T ?K) =>
       apply (proj43 (type_equal_core_validated_inv H))
   end : type_equal_core_validated.
 
-Hint Extern 1 (valid_kind ?E ?K) =>
+Hint Extern 1 (valid_kind_validated ?E ?K) =>
   match goal with
   | H : type_equal_core_validated E _ _ K |- _ =>
       apply (proj44 (type_equal_core_validated_inv H))
   end : type_equal_core_validated.
 
+Hint Extern 1 (valid_env ?E) =>
+  match goal with
+  | H : type_equal_core_validated E _ _ _ |- _ =>
+      apply (unvalidated_valid_env
+               (proj41 (type_equal_core_validated_inv H)))
+  end : type_equal_core_regular.
+
+Hint Extern 1 (kinding ?E ?T ?K) =>
+  match goal with
+  | H : type_equal_core_validated E T _ K |- _ =>
+      apply (unvalidated_kinding
+               (proj42 (type_equal_core_validated_inv H)))
+  | H : type_equal_core_validated E _ T K |- _ =>
+      apply (unvalidated_kinding
+               (proj43 (type_equal_core_validated_inv H)))
+  end : type_equal_core_validated.
+
+Hint Extern 1 (valid_kind ?E ?K) =>
+  match goal with
+  | H : type_equal_core_validated E _ _ K |- _ =>
+      apply (unvalidated_valid_kind
+               (proj44 (type_equal_core_validated_inv H)))
+  end : type_equal_core_validated.
+
 Lemma type_equal_cong_validated_inv : forall E T1 T2 K,
     type_equal_cong_validated E T1 T2 K ->
-    valid_env E /\ kinding E T1 K /\ kinding E T2 K /\ valid_kind E K.
+    valid_env_validated E
+    /\ kinding_validated E T1 K
+    /\ kinding_validated E T2 K
+    /\ valid_kind_validated E K.
 Proof.
   introv Hte.
-  destruct Hte; splits; auto with csetdec; eauto.
-  - apply kinding_range_subsumption with (T1 := T1') (T2 := T1');
-      auto.
-    + apply raw_subtype_reflexive_equal; eauto.
-    + apply raw_subtype_reflexive_equal; eauto.
-  - auto using raw_subtype_reflexive.
+  destruct Hte; splits;
+    auto with valid_kind_validated kinding_validated csetdec;
+    eauto with kinding_validated.
 Qed.
 
 Hint Constructors type_equal_cong_validated
@@ -2816,13 +2819,13 @@ Hint Extern 1 (CSet.Nonempty ?cs) =>
       inversion Hknd; assumption
   end : type_equal_cong_regular.
 
-Hint Extern 1 (valid_env ?E) =>
+Hint Extern 1 (valid_env_validated ?E) =>
   match goal with
   | H : type_equal_cong_validated E _ _ _ |- _ =>
       apply (proj41 (type_equal_cong_validated_inv H))
-  end : type_equal_cong_regular.
+  end : type_equal_cong_validated.
 
-Hint Extern 1 (kinding ?E ?T ?K) =>
+Hint Extern 1 (kinding_validated ?E ?T ?K) =>
   match goal with
   | H : type_equal_cong_validated E T _ K |- _ =>
       apply (proj42 (type_equal_cong_validated_inv H))
@@ -2830,15 +2833,42 @@ Hint Extern 1 (kinding ?E ?T ?K) =>
       apply (proj43 (type_equal_cong_validated_inv H))
   end : type_equal_cong_validated.
 
-Hint Extern 1 (valid_kind ?E ?K) =>
+Hint Extern 1 (valid_kind_validated ?E ?K) =>
   match goal with
   | H : type_equal_cong_validated E _ _ K |- _ =>
       apply (proj44 (type_equal_cong_validated_inv H))
   end : type_equal_cong_validated.
 
+Hint Extern 1 (valid_env ?E) =>
+  match goal with
+  | H : type_equal_cong_validated E _ _ _ |- _ =>
+      apply (unvalidated_valid_env
+               (proj41 (type_equal_cong_validated_inv H)))
+  end : type_equal_cong_regular.
+
+Hint Extern 1 (kinding ?E ?T ?K) =>
+  match goal with
+  | H : type_equal_cong_validated E T _ K |- _ =>
+      apply (unvalidated_kinding
+               (proj42 (type_equal_cong_validated_inv H)))
+  | H : type_equal_cong_validated E _ T K |- _ =>
+      apply (unvalidated_kinding
+               (proj43 (type_equal_cong_validated_inv H)))
+  end : type_equal_cong_validated.
+
+Hint Extern 1 (valid_kind ?E ?K) =>
+  match goal with
+  | H : type_equal_cong_validated E _ _ K |- _ =>
+      apply (unvalidated_valid_kind
+               (proj44 (type_equal_cong_validated_inv H)))
+  end : type_equal_cong_validated.
+
 Lemma type_equal_symm_validated_inv : forall E T1 T2 K,
     type_equal_symm_validated E T1 T2 K ->
-    valid_env E /\ kinding E T1 K /\ kinding E T2 K /\ valid_kind E K.
+    valid_env_validated E
+    /\ kinding_validated E T1 K
+    /\ kinding_validated E T2 K
+    /\ valid_kind_validated E K.
 Proof.
   introv Hte.
   destruct Hte; auto.
@@ -2881,13 +2911,13 @@ Hint Extern 1 (CSet.Nonempty ?cs) =>
       inversion Hknd; assumption
   end : type_equal_symm_regular.
 
-Hint Extern 1 (valid_env ?E) =>
+Hint Extern 1 (valid_env_validated ?E) =>
   match goal with
   | H : type_equal_symm_validated E _ _ _ |- _ =>
       apply (proj41 (type_equal_symm_validated_inv H))
-  end : type_equal_symm_regular.
+  end : type_equal_symm_validated.
 
-Hint Extern 1 (kinding ?E ?T ?K) =>
+Hint Extern 1 (kinding_validated ?E ?T ?K) =>
   match goal with
   | H : type_equal_symm_validated E T _ K |- _ =>
       apply (proj42 (type_equal_symm_validated_inv H))
@@ -2895,15 +2925,42 @@ Hint Extern 1 (kinding ?E ?T ?K) =>
       apply (proj43 (type_equal_symm_validated_inv H))
   end : type_equal_symm_validated.
 
-Hint Extern 1 (valid_kind ?E ?K) =>
+Hint Extern 1 (valid_kind_validated ?E ?K) =>
   match goal with
   | H : type_equal_symm_validated E _ _ K |- _ =>
       apply (proj44 (type_equal_symm_validated_inv H))
   end : type_equal_symm_validated.
 
+Hint Extern 1 (valid_env ?E) =>
+  match goal with
+  | H : type_equal_symm_validated E _ _ _ |- _ =>
+      apply (unvalidated_valid_env
+               (proj41 (type_equal_symm_validated_inv H)))
+  end : type_equal_symm_regular.
+
+Hint Extern 1 (kinding ?E ?T ?K) =>
+  match goal with
+  | H : type_equal_symm_validated E T _ K |- _ =>
+      apply (unvalidated_kinding
+               (proj42 (type_equal_symm_validated_inv H)))
+  | H : type_equal_symm_validated E _ T K |- _ =>
+      apply (unvalidated_kinding
+               (proj43 (type_equal_symm_validated_inv H)))
+  end : type_equal_symm_validated.
+
+Hint Extern 1 (valid_kind ?E ?K) =>
+  match goal with
+  | H : type_equal_symm_validated E _ _ K |- _ =>
+      apply (unvalidated_valid_kind
+               (proj44 (type_equal_symm_validated_inv H)))
+  end : type_equal_symm_validated.
+
 Lemma type_equal_validated_inv : forall E T1 T2 K,
     type_equal_validated E T1 T2 K ->
-    valid_env E /\ kinding E T1 K /\ kinding E T2 K /\ valid_kind E K.
+    valid_env_validated E
+    /\ kinding_validated E T1 K
+    /\ kinding_validated E T2 K
+    /\ valid_kind_validated E K.
 Proof.
   introv Hk.
   destruct Hk; auto.
@@ -2945,13 +3002,13 @@ Hint Extern 1 (CSet.Nonempty ?cs) =>
       inversion Hknd; assumption
   end : type_equal_regular.
 
-Hint Extern 1 (valid_env ?E) =>
+Hint Extern 1 (valid_env_validated ?E) =>
   match goal with
   | H : type_equal_validated E _ _ _ |- _ =>
       apply (proj41 (type_equal_validated_inv H))
-  end : type_equal_regular.
+  end : type_equal_validated.
 
-Hint Extern 1 (kinding ?E ?T ?K) =>
+Hint Extern 1 (kinding_validated ?E ?T ?K) =>
   match goal with
   | H : type_equal_validated E T _ K |- _ =>
       apply (proj42 (type_equal_validated_inv H))
@@ -2959,16 +3016,41 @@ Hint Extern 1 (kinding ?E ?T ?K) =>
       apply (proj43 (type_equal_validated_inv H))
   end : type_equal_validated.
 
-Hint Extern 1 (valid_kind ?E ?K) =>
+Hint Extern 1 (valid_kind_validated ?E ?K) =>
   match goal with
   | H : type_equal_validated E _ _ K |- _ =>
       apply (proj44 (type_equal_validated_inv H))
   end : type_equal_validated.
 
+Hint Extern 1 (valid_env ?E) =>
+  match goal with
+  | H : type_equal_validated E _ _ _ |- _ =>
+      apply (unvalidated_valid_env
+               (proj41 (type_equal_validated_inv H)))
+  end : type_equal_regular.
+
+Hint Extern 1 (kinding ?E ?T ?K) =>
+  match goal with
+  | H : type_equal_validated E T _ K |- _ =>
+      apply (unvalidated_kinding
+               (proj42 (type_equal_validated_inv H)))
+  | H : type_equal_validated E _ T K |- _ =>
+      apply (unvalidated_kinding
+               (proj43 (type_equal_validated_inv H)))
+  end : type_equal_validated.
+
+Hint Extern 1 (valid_kind ?E ?K) =>
+  match goal with
+  | H : type_equal_validated E _ _ K |- _ =>
+      apply (unvalidated_valid_kind
+               (proj44 (type_equal_validated_inv H)))
+  end : type_equal_validated.
+
 Lemma subtype_validated_inv : forall E T1 T2 cs,
     subtype_validated E T1 T2 cs ->
-    valid_env E
-    /\ kinding E T1 (knd_row cs) /\ kinding E T2 (knd_row cs).
+    valid_env_validated E
+    /\ kinding_validated E T1 (knd_row cs)
+    /\ kinding_validated E T2 (knd_row cs).
 Proof.
   introv Hk.
   destruct Hk; auto.
@@ -3000,13 +3082,13 @@ Hint Extern 1 (CSet.Nonempty ?cs) =>
         (regular_subtype (unvalidated_subtype H))))
   end : subtype_regular.
 
-Hint Extern 1 (valid_env ?E) =>
+Hint Extern 1 (valid_env_validated ?E) =>
   match goal with
   | H : subtype_validated E _ _ _ |- _ =>
       apply (proj31 (subtype_validated_inv H))
   end : subtype_validated.
 
-Hint Extern 1 (kinding ?E ?T (knd_row ?cs)) =>
+Hint Extern 1 (kinding_validated ?E ?T (knd_row ?cs)) =>
   match goal with
   | H : subtype_validated E T _ cs |- _ =>
       apply (proj32 (subtype_validated_inv H))
@@ -3014,52 +3096,426 @@ Hint Extern 1 (kinding ?E ?T (knd_row ?cs)) =>
       apply (proj33 (subtype_validated_inv H))
   end : subtype_validated.
 
-Lemma validated_combined_kinding :
-  (forall E K, valid_kind E K -> valid_kind_validated E K)
-  /\ (forall E T K, kinding E T K -> kinding_validated E T K)
-  /\ (forall E M Xs,
-         valid_scheme_vars E M Xs -> valid_scheme_vars_validated E M Xs)
-  /\ (forall E M, valid_scheme E M -> valid_scheme_validated E M)
-  /\ (forall E, valid_env E -> valid_env_validated E)
-  /\ (forall E T1 T2 K,
-       type_equal_core E T1 T2 K -> type_equal_core_validated E T1 T2 K)
-  /\ (forall E T1 T2 K,
-       type_equal_cong E T1 T2 K -> type_equal_cong_validated E T1 T2 K)
-  /\ (forall E T1 T2 K,
-       type_equal_symm E T1 T2 K -> type_equal_symm_validated E T1 T2 K)
-  /\ (forall E T1 T2 K,
-       type_equal E T1 T2 K -> type_equal_validated E T1 T2 K)
-  /\ (forall E T1 T2 cs,
-       subtype E T1 T2 cs -> subtype_validated E T1 T2 cs).
+Hint Extern 1 (valid_env ?E) =>
+  match goal with
+  | H : subtype_validated E _ _ _ |- _ =>
+      apply (unvalidated_valid_env (proj31 (subtype_validated_inv H)))
+  end : subtype_validated.
+
+Hint Extern 1 (kinding ?E ?T (knd_row ?cs)) =>
+  match goal with
+  | H : subtype_validated E T _ cs |- _ =>
+      apply (unvalidated_kinding (proj32 (subtype_validated_inv H)))
+  | H : subtype_validated E _ T cs |- _ =>
+      apply (unvalidated_kinding (proj33 (subtype_validated_inv H)))
+  end : subtype_validated.
+
+Lemma combined_kinding_validated_weakening :
+     (forall EG K,
+      valid_kind_validated EG K ->
+      (forall E F G,
+          EG = E & G ->
+          valid_env_validated (E & F & G) ->
+          valid_kind_validated (E & F & G) K))
+  /\ (forall EG T K,
+      kinding_validated EG T K ->
+      (forall E F G,
+          EG = E & G ->
+          valid_env_validated (E & F & G) ->
+          kinding_validated (E & F & G) T K))
+  /\ (forall EG M Xs,
+      valid_scheme_vars_validated EG M Xs ->
+      (forall E F G,
+          fresh (dom F) (sch_arity M) Xs ->
+          EG = E & G ->
+          valid_env_validated (E & F & G) ->
+          valid_scheme_vars_validated (E & F & G) M Xs))
+  /\ (forall EG M,
+      valid_scheme_validated EG M ->
+      (forall E F G,
+          EG = E & G ->
+          valid_env_validated (E & F & G) ->
+          valid_scheme_validated (E & F & G) M))
+  /\ (forall EGX,
+      valid_env_validated EGX ->
+      (forall E F G X K,
+          X # F ->
+          EGX = E & G & X ~:: K ->
+          valid_env_validated (E & F & G) ->
+          valid_env_validated (E & F & G & X ~:: K)))
+  /\ (forall EG T1 T2 K,
+      type_equal_core_validated EG T1 T2 K ->
+      (forall E F G,
+          EG = E & G ->
+          valid_env_validated (E & F & G) ->
+          type_equal_core_validated (E & F & G) T1 T2 K))
+  /\ (forall EG T1 T2 K,
+      type_equal_cong_validated EG T1 T2 K ->
+      (forall E F G,
+          EG = E & G ->
+          valid_env_validated (E & F & G) ->
+          type_equal_cong_validated (E & F & G) T1 T2 K))
+  /\ (forall EG T1 T2 K,
+      type_equal_symm_validated EG T1 T2 K ->
+      (forall E F G,
+          EG = E & G ->
+          valid_env_validated (E & F & G) ->
+          type_equal_symm_validated (E & F & G) T1 T2 K))
+  /\ (forall EG T1 T2 K,
+      type_equal_validated EG T1 T2 K ->
+      (forall E F G,
+          EG = E & G ->
+          valid_env_validated (E & F & G) ->
+          type_equal_validated (E & F & G) T1 T2 K))
+  /\ (forall EG T1 T2 cs,
+      subtype_validated EG T1 T2 cs ->
+      (forall E F G,
+          EG = E & G ->
+          valid_env_validated (E & F & G) ->
+          subtype_validated (E & F & G) T1 T2 cs)).
 Proof.
-  apply combined_kinding_mutind; intros; subst;
+  apply combined_kinding_validated_mutind;
+    intros; subst; econstr auto with valid_env_regular.
+  - auto using binds_weakening
+      with kinding_validated valid_env_validated valid_env_regular.
+  - apply kinding_validated_variant with (T1 := T1) (T2 := T2);
+      auto with valid_env_regular.
+  - apply kinding_validated_range_subsumption
+      with (T1 := T1) (T2 := T2);
+      auto with valid_env_regular.
+  - assert (fresh (dom F) (sch_arity (sch_bind K M)) (X :: Xs)) as Hf
+        by assumption.
+    destruct Hf.
+    apply valid_scheme_vars_validated_bind;
+      auto using environment_knd_weakening with valid_env_regular.
+    rewrite <- concat_assoc.
+    apply H0;
+      autorewrite with rew_sch_arity; rewrite? concat_assoc; auto.
+  - apply valid_scheme_validated_c
+      with (L := (L \u dom F)); auto with valid_env_regular.
+  - exfalso. eauto using empty_push_inv.
+  - destruct (eq_push_inv H2) as [? [Heq ?]].
+    inversion Heq; subst.
+    auto with valid_env_validated valid_env_regular.
+  - destruct (eq_push_inv H2) as [_ [? _]].
+    discriminate.
+  - apply type_equal_core_validated_or_associative
+      with (cs1 := cs1) (cs2 := cs2) (cs3 := cs3);
+      auto with valid_env_regular.
+  - apply type_equal_cong_validated_variant
+      with (T2 := T2) (T3 := T3); auto with valid_env_regular.
+  - apply type_equal_cong_validated_range_subsumption
+      with (T3 := T3) (T4 := T4); auto with valid_env_regular.
+  - apply type_equal_validated_step with (T2 := T2);
+      auto with valid_env_regular.
+Qed.
+
+Lemma valid_kind_validated_weakening : forall E F G K,
+    valid_kind_validated (E & G) K ->
+    valid_env_validated (E & F & G) ->
+    valid_kind_validated (E & F & G) K.
+Proof.
+  pose combined_kinding_validated_weakening.
+  intuition eauto.
+Qed.
+
+Lemma valid_kind_validated_from_env : forall E X K,
+    valid_env_validated E ->
+    binds X (bind_knd K) E ->
+    valid_kind_validated E K.
+Proof.
+  introv He Hb.
+  induction He.
+  - apply binds_empty_inv in Hb; contradiction.
+  - destruct (binds_push_inv Hb) as [[Hx Hbnd]|[Hx Hbnd]];
+      inversion Hbnd; subst;
+      rewrite <- concat_empty_r with (E := E & X0 ~:: K0);
+      apply valid_kind_validated_weakening;
+      rewrite concat_empty_r; auto with valid_env_validated.
+  - destruct (binds_push_inv Hb) as [[Hx Hbnd]|[Hx Hbnd]];
+      try discriminate.
+    rewrite <- concat_empty_r with (E := E & x ~: M).
+    apply valid_kind_validated_weakening;
+      rewrite concat_empty_r; auto with valid_env_validated.
+Qed.
+
+Lemma type_equal_validated_reflexive : forall E T K,
+    kinding_validated E T K ->
+    type_equal_validated E T T K.
+Proof.
+  intros.
+  auto using type_equal_validated_refl
+    with kinding_regular kinding_validated.
+Qed.
+
+Lemma type_equal_validated_transitive : forall E T1 T2 T3 K,
+    type_equal_validated E T1 T2 K ->
+    type_equal_validated E T2 T3 K ->
+    type_equal_validated E T1 T3 K.
+Proof.
+  introv Hte1 Hte2.
+  induction Hte1;
+    eauto using type_equal_validated
+      with type_equal_regular type_equal_validated.
+Qed.
+
+Lemma type_equal_symm_validated_symmetric : forall E T1 T2 K,
+    type_equal_symm_validated E T1 T2 K ->
+    type_equal_symm_validated E T2 T1 K.
+Proof.
+  introv Hte.
+  induction Hte; auto using type_equal_symm_validated.
+Qed.
+
+Lemma type_equal_validated_symmetric_ind : forall E T1 T2 T3 K,
+    type_equal_validated E T2 T1 K ->
+    type_equal_validated E T2 T3 K ->
+    type_equal_validated E T3 T1 K.
+Proof.
+  introv Hacc Hte.
+  induction Hte;
+    eauto using type_equal_symm_validated_symmetric
+      with type_equal_validated type_equal_regular.
+Qed.
+
+Lemma type_equal_validated_symmetric : forall E T1 T2 K,
+    type_equal_validated E T1 T2 K ->
+    type_equal_validated E T2 T1 K.
+Proof.
+  introv Hte.
+  apply type_equal_validated_symmetric_ind with (T2 := T1);
+    try assumption.
+  apply type_equal_validated_refl;
+    auto with type_equal_regular type_equal_validated.
+Qed.
+
+Lemma subtype_validated_reflexive : forall E T cs,
+    kinding_validated E T (knd_row cs) ->
+    subtype_validated E T T cs.
+Proof.
+  introv Hk.
+  apply subtype_validated_c;
+    auto with kinding_regular kinding_validated.
+  apply type_equal_validated_step
+    with (T2 := (typ_meet T (typ_join T (typ_bot cs))));
+    auto 6 with kinding_regular kinding_validated
+      type_equal_symm_validated type_equal_cong_validated
+      type_equal_core_validated.
+  apply type_equal_validated_step
+    with (T2 := (typ_meet T T));
+    auto 6 with kinding_regular kinding_validated
+      type_equal_symm_validated type_equal_cong_validated
+      type_equal_core_validated.
+  apply type_equal_validated_refl;
+    auto with kinding_regular kinding_validated.
+Qed.
+
+Lemma type_equal_validated_meet_r : forall E T1 T2 T2' cs,
+    kinding_validated E T1 (knd_row cs) ->
+    type_equal_validated E T2 T2' (knd_row cs) ->
+    type_equal_validated E
+      (typ_meet T1 T2) (typ_meet T1 T2') (knd_row cs).
+Proof.
+  introv Hk Hte.
+  remember (knd_row cs).
+  induction Hte; subst.
+  - apply type_equal_validated_refl;
+      auto with kinding_regular kinding_validated.
+  - apply type_equal_validated_step
+      with (T2 := typ_meet T1 T2);
+      auto with kinding_regular kinding_validated.
+    assert (type_equal_symm_validated E T0 T2 (knd_row cs)) as Htes
+      by assumption.
+    remember (knd_row cs).
+    destruct Htes; subst;
+      auto with kinding_regular kinding_validated
+        type_equal_symm_validated type_equal_cong_validated.
+Qed.
+
+Lemma type_equal_validated_meet_l : forall E T1 T1' T2 cs,
+    kinding_validated E T2 (knd_row cs) ->
+    type_equal_validated E T1 T1' (knd_row cs) ->
+    type_equal_validated E
+      (typ_meet T1 T2) (typ_meet T1' T2) (knd_row cs).
+Proof.
+  introv Hk Hte.
+  remember (knd_row cs).
+  induction Hte; subst.
+  - apply type_equal_validated_refl;
+      auto with kinding_regular kinding_validated.
+  - apply type_equal_validated_step
+      with (T2 := typ_meet T0 T2);
+      auto with kinding_regular kinding_validated.
+    assert (type_equal_symm_validated E T1 T0 (knd_row cs)) as Htes
+      by assumption.
+    remember (knd_row cs).
+    destruct Htes; subst;
+      auto with kinding_regular kinding_validated
+        type_equal_symm_validated type_equal_cong_validated.
+Qed.
+
+Lemma type_equal_validated_meet_idempotent : forall E T cs,
+    kinding_validated E T (knd_row cs) ->
+    type_equal_validated E T (typ_meet T T) (knd_row cs).
+Proof.
+  introv Hk.
+  apply type_equal_validated_step
+    with (T2 := typ_meet T (typ_join T (typ_bot cs)));
+    auto 6 with kinding_regular kinding_validated
+      type_equal_symm_validated type_equal_cong_validated
+      type_equal_core_validated.
+  apply type_equal_validated_step
+    with (T2 := typ_meet T T);
+    auto 6 with kinding_regular kinding_validated
+      type_equal_symm_validated type_equal_cong_validated
+      type_equal_core_validated.
+  apply type_equal_validated_refl;
+    auto with kinding_regular kinding_validated.
+Qed.
+     
+Lemma subtype_validated_transitive : forall E T1 T2 T3 cs,
+    subtype_validated E T1 T2 cs ->
+    subtype_validated E T2 T3 cs ->
+    subtype_validated E T1 T3 cs.
+Proof.
+  introv Hs1 Hs2.
+  apply subtype_validated_c;
+    auto with subtype_regular subtype_validated.
+  destruct Hs1. destruct Hs2.
+  apply type_equal_validated_transitive
+    with (T2 := typ_meet T1 T0); auto.
+  apply type_equal_validated_transitive
+    with (T2 := typ_meet T1 (typ_meet T0 T2));
+    auto using type_equal_validated_meet_r.
+  apply type_equal_validated_step
+    with (T2 := typ_meet (typ_meet T1 T0) T2);
+    auto with kinding_regular kinding_validated
+      type_equal_symm_validated type_equal_cong_validated
+      type_equal_core_validated.
+  apply type_equal_validated_transitive with (T2 := typ_meet T1 T2);
+    auto using type_equal_validated_meet_l,
+      type_equal_validated_reflexive,
+      type_equal_validated_symmetric.
+Qed.
+
+Lemma subtype_validated_antisymmetric : forall E T1 T2 cs,
+    subtype_validated E T1 T2 cs ->
+    subtype_validated E T2 T1 cs ->
+    type_equal_validated E T1 T2 (knd_row cs).
+Proof.
+  introv Hs1 Hs2.
+  destruct Hs1. destruct Hs2.
+  apply type_equal_validated_transitive
+    with (T2 := typ_meet T2 T1); auto.
+  apply type_equal_validated_step
+    with (T2 := typ_meet T1 T2);
+    auto with kinding_regular kinding_validated
+      type_equal_symm_validated type_equal_cong_validated
+      type_equal_core_validated.
+  apply type_equal_validated_symmetric; auto.
+Qed.
+
+Lemma subtype_validated_reflexive_equal : forall E T1 T2 cs,
+    type_equal_validated E T1 T2 (knd_row cs) ->
+    subtype_validated E T1 T2 cs.
+Proof.
+  introv Hte.
+  apply subtype_validated_c;
+    auto with type_equal_regular type_equal_validated.
+  apply type_equal_validated_transitive with (T2 := typ_meet T1 T1);
+    auto using type_equal_validated_meet_idempotent
+      with type_equal_validated.
+  auto using type_equal_validated_meet_r
+    with type_equal_validated.
+Qed.
+
+Lemma validated_combined_kinding_regular :
+  (forall E K, valid_kind_regular E K -> valid_kind_validated E K)
+  /\ (forall E T K, kinding_regular E T K -> kinding_validated E T K)
+  /\ (forall E M Xs,
+         valid_scheme_vars_regular E M Xs ->
+         valid_scheme_vars_validated E M Xs)
+  /\ (forall E M, valid_scheme_regular E M ->
+                  valid_scheme_validated E M)
+  /\ (forall E, valid_env_regular E -> valid_env_validated E)
+  /\ (forall E T1 T2 K,
+       type_equal_core_regular E T1 T2 K ->
+       type_equal_core_validated E T1 T2 K)
+  /\ (forall E T1 T2 K,
+       type_equal_cong_regular E T1 T2 K ->
+       type_equal_cong_validated E T1 T2 K)
+  /\ (forall E T1 T2 K,
+       type_equal_symm_regular E T1 T2 K ->
+       type_equal_symm_validated E T1 T2 K)
+  /\ (forall E T1 T2 K,
+       type_equal_regular E T1 T2 K -> type_equal_validated E T1 T2 K)
+  /\ (forall E T1 T2 cs,
+       subtype_regular E T1 T2 cs -> subtype_validated E T1 T2 cs).
+Proof.
+  apply combined_kinding_regular_mutind; intros; subst;
     econstr auto with valid_kind_validated kinding_validated
            valid_scheme_vars_validated valid_scheme_validated
            valid_env_validated type_equal_core_validated
            type_equal_cong_validated type_equal_symm_validated
            type_equal_validated subtype_validated.
-  - assert (environment E) by auto with valid_env_validated.
-    assert (kind K) by (eapply kind_from_env; eassumption).
+  - assert (valid_env_validated E) by auto with valid_env_validated.
+    assert (valid_kind_validated E K)
+      by (eapply valid_kind_validated_from_env; eassumption).   
     auto with kinding_validated.
-  - assert (kind (knd_range T1 T2)) as Hknd
+  - auto using subtype_validated_reflexive
+      with valid_kind_validated kinding_regular kinding_validated.
+  - assert (valid_kind_validated E (knd_range T1 T2)) as Hknd
       by auto with kinding_validated.
     inversion Hknd; subst.
     apply kinding_validated_variant with (T1 := T1) (T2 := T2);
       auto with kinding_validated.
+  - assert (valid_kind_validated E (knd_range T1 T2)) as Hknd
+      by auto with kinding_validated.
+    inversion Hknd; subst.
+    assert (subtype_validated E T2' T1' CSet.universe)
+      by eauto using subtype_validated_transitive.
+    apply kinding_validated_range_subsumption
+      with (T1 := T1) (T2 := T2);
+      auto with subtype_validated valid_kind_validated.
   - apply valid_scheme_validated_c with (L := L); try assumption.
-    + pick_freshes_gen L (sch_arity M) Xs.
-      assert (valid_scheme_vars_validated E M Xs) by auto.
-      auto with valid_scheme_vars_validated.
-    + exists L. intros.
-      assert (valid_scheme_vars_validated E M Xs) by auto.
-      auto with valid_scheme_vars_validated.
-  - assert (kind (knd_range T2 T3)) as Hknd
+    pick_freshes_gen L (sch_arity M) Xs.
+    assert (valid_scheme_vars_validated E M Xs) by auto.
+    auto with valid_scheme_vars_validated.
+  - assert (subtype_validated E T1' T1' CSet.universe)
+      by auto using subtype_validated_reflexive
+           with type_equal_cong_validated.
+    assert (subtype_validated E T1 T1 CSet.universe)
+      by auto using subtype_validated_reflexive
+           with type_equal_cong_validated.
+    assert (subtype_validated E T1 T1' CSet.universe)
+      by eauto using subtype_validated_reflexive_equal
+           with type_equal_validated type_equal_symm_validated
+             type_equal_cong_regular type_equal_cong_validated.
+    assert (subtype_validated E T1' T1 CSet.universe)
+      by eauto using subtype_validated_reflexive_equal
+           with type_equal_validated type_equal_symm_validated
+             type_equal_cong_regular type_equal_cong_validated.
+    apply type_equal_cong_validated_row;
+      auto with valid_kind_validated type_equal_cong_validated.
+    apply kinding_validated_range_subsumption
+      with (T1 := T1') (T2 := T1');
+      auto with valid_kind_validated kinding_validated
+        type_equal_cong_regular type_equal_cong_validated.
+  - assert (valid_kind_validated E (knd_range T2 T3)) as Hknd
       by auto with type_equal_cong_validated.
     inversion Hknd; subst.
-    auto with type_equal_cong_validated.
-  - assert (type (typ_meet T1 T2)) as Ht
+    eauto with type_equal_cong_validated.
+  - assert (valid_kind_validated E (knd_range T3 T4)) as Hknd
+      by auto with type_equal_cong_validated.
+    inversion Hknd; subst.
+    assert (subtype_validated E T4' T3' CSet.universe)
+      by eauto using subtype_validated_transitive.
+    econstructor; try eassumption;
+      auto with valid_kind_validated
+        type_equal_cong_validated subtype_validated.
+  - assert (kinding_validated E (typ_meet T1 T2) (knd_row cs)) as Hk
       by auto with type_equal_validated.
-    inversion Ht; subst.
+    inversion Hk; subst.
     auto with subtype_validated type_equal_validated.
 Qed.
 
